examples/byte_register.thy
@@ -17,22 +17,22 @@ unbundle Expression_Syntax
 type_synonym bit = "1 word"
 
 alphabet \<alpha>ST = 
-  reg :: "8 word"
+  reg :: nat
   err :: bit
 
 alphabet \<alpha>H =
-  reg\<^sub>H :: "4 word"
+  reg\<^sub>H :: nat
   err\<^sub>H :: bit
 
 alphabet \<alpha>L =
-  reg\<^sub>L :: "4 word"
+  reg\<^sub>L :: nat
   err\<^sub>L :: bit
 
 (* ST defines what states are valid *)
-(*
+
 definition ST
   where "ST = (reg \<ge> 0 \<and> reg \<le> 255 \<and> err \<ge> 0 \<and> err \<le> 1)\<^sub>e"
-*)
+
 
 (* DBL doubles the number, if it is low enough to double without overflow *)
 definition DBL
@@ -47,24 +47,18 @@ lemma DBL_design: "DBL = ((reg\<^sup>< \<ge> 0 \<and> reg\<^sup>< \<le> 127 \<an
 
 (* A view of the high nibble *)
 definition Hv
-  where "Hv = OK (((vu:reg\<^sub>H = (ucast (drop_bit 4 sys:reg))) \<and> (vu:err\<^sub>H = sys:err))\<^sub>e \<up> \<^bold>v\<^sub>D)"
+  where "Hv = ((vu:reg\<^sub>H = (drop_bit 4 sys:reg)) \<and> (vu:err\<^sub>H = sys:err))\<^sub>e"
 
 (* A view of the low nibble *)
 definition Lv
-  where "Lv = OK (((vu:reg\<^sub>L = (ucast (take_bit 4 sys:reg))) \<and> (vu:err\<^sub>L = sys:err))\<^sub>e \<up> \<^bold>v\<^sub>D)"
+  where "Lv = ((vu:reg\<^sub>L = (take_bit 4 sys:reg)) \<and> (vu:err\<^sub>L = sys:err))\<^sub>e"
 
 (* These are both healthy *)
-lemma hv_is_vhd: "Hv is VHD"
+lemma hv_is_vhd: "Hv is VH"
   by (pred_auto_banks add: Hv_def)
 
-lemma lv_is_vhd: "Lv is VHD"
-  by (pred_auto_banks add: Lv_def)
-
-lemma ok_free_hv: "$ok \<sharp> Hv"
-  by (pred_auto_banks add: Hv_def)
-
-lemma ok_free_lv: "$ok \<sharp> Lv"
-  by (pred_auto_banks add: Lv_def)
+lemma lv_is_vhd: "Lv is VH"
+  by (pred_auto_banks add: Lv_def) 
 
 (*
 Consider an example where the register stores the value 60
@@ -83,27 +77,59 @@ definition \<Phi> where "\<Phi> = (reg = 60 \<and> err = 0)\<^sub>e"
       LLLL = 1100(b2) = 12(b10)
 *)
 
-lemma "(((L (Hv \<down> \<^bold>v\<^sub>D) (\<Delta> \<Phi>))) \<down> vu\<^sup>2) = \<Delta> (reg\<^sub>H = 3 \<and> err\<^sub>H = 0)\<^sub>e"
+lemma "(((L (Hv) (\<Delta> \<Phi>))) \<down> vu\<^sup>2) = \<Delta> (reg\<^sub>H = 3 \<and> err\<^sub>H = 0)\<^sub>e"
   by (pred_auto_banks add: Hv_def \<Phi>_def)
 
-lemma "(((L (Lv \<down> \<^bold>v\<^sub>D) (\<Delta> \<Phi>))) \<down> vu\<^sup>2) = \<Delta> (reg\<^sub>L = 12 \<and> err\<^sub>L = 0)\<^sub>e"
+lemma "(((L (Lv) (\<Delta> \<Phi>))) \<down> vu\<^sup>2) = \<Delta> (reg\<^sub>L = 12 \<and> err\<^sub>L = 0)\<^sub>e"
   by (pred_auto_banks add: Lv_def \<Phi>_def)
 
 definition Loc_H_DBL where "Loc_H_DBL = (L\<^sub>D (Hv) (DBL))"
 definition Loc_L_DBL where "Loc_L_DBL = (L\<^sub>D (Lv) (DBL))"
 
 
-(* this might turn out to be useful *)
-lemma drop_word_lt_div: "(r :: 8 word) \<le> a \<longrightarrow> (drop_bit k r) \<le> a div 2^k"
+lemma drop_8word_lt_div:
+  assumes "(r :: 8 word) \<le> a"
+  shows "(drop_bit k r) \<le> a div 2^k"
+  using assms
   by (simp add: drop_bit_eq_div word_le_nat_alt unat_div_distrib div_le_mono)
 
+lemma drop_8word_lt_div_inv:
+  assumes "(drop_bit k r) < a div 2^k"
+  shows "(r :: 8 word) < a"
+  using assms
+  by (metis drop_8word_lt_div drop_bit_eq_div linorder_not_less)
 
-lemma "Loc_L_DBL = ((L\<^sub>D (Lv) (((reg\<^sup>< \<ge> 0 \<and> reg\<^sup>< \<le> 127 \<and> err\<^sup>< = 0)\<^sub>e \<up> \<^bold>v\<^sub>D\<^sup>2) \<turnstile> ((reg\<^sup>> = reg\<^sup>< * 2 \<and> err\<^sup>> = 0)\<^sub>e \<up> \<^bold>v\<^sub>D\<^sup>2))))"
-  by (pred_auto_banks add: Loc_L_DBL_def DBL_def)
+lemma drop_4_8_128:
+  assumes "drop_bit 4 r < (8::8 word)"
+  shows "r < 128"
+proof -
+  have expand_8: "(8 :: 8 word) = (128 div (2^4))" by simp
+  from assms show ?thesis
+    apply (subst (asm) expand_8)
+    by (erule_tac drop_8word_lt_div_inv)
+qed
 
+lemma le_to_lt127: "(x \<le> (127 :: 8 word)) = (x < (128 :: 8 word))"
+   apply transfer
+   by auto
+
+lemma le_to_lt7: "(x \<le> (7 :: 8 word)) = (x < (8 :: 8 word))"
+   apply transfer
+   by auto
+
+lemma drop_4_le_7_127:
+  assumes "drop_bit 4 r \<le> (7::8 word)"
+  shows "r \<le> (127 :: 8 word)"
+  using assms
+  apply (subst le_to_lt127)
+  apply (subst (asm) le_to_lt7)
+  apply (simp add: assms drop_4_8_128)
+  dones
+
+declare [[smt_trace = true]]
 declare [[smt_oracle = true]]
-declare [[z3_extensions = true]]
 
+(*
 lemma loc_l_dbl_simp: "Loc_L_DBL = ((\<not>L\<^sub>D (Lv) (\<not> ((reg\<^sup>< \<ge> 0 \<and> reg\<^sup>< \<le> 127 \<and> err\<^sup>< = 0)\<^sub>e  \<up> \<^bold>v\<^sub>D\<^sup>2)))) \<turnstile> ((L\<^sub>D (Lv) ((reg\<^sup>> = reg\<^sup>< * 2 \<and> err\<^sup>> = 0)\<^sub>e \<up> \<^bold>v\<^sub>D\<^sup>2)))"
   by (pred_auto_banks add: Lv_def DBL_def Loc_L_DBL_def)
 
@@ -113,25 +139,74 @@ lemma "Loc_H_DBL = ((\<not>L\<^sub>D (Hv) (\<not> ((reg\<^sup>< \<ge> 0 \<and> r
 lemma "Loc_L_DBL = true"
   apply (pred_auto_banks add: Lv_def DBL_def Loc_L_DBL_def)
   by smt
+*)
 
+lemma loc_l_dbl_simp: "Loc_L_DBL = 
+    (\<not>L (Lv) (\<not> ((reg\<^sup>< \<ge> 0 \<and> reg\<^sup>< \<le> 127 \<and> err\<^sup>< = 0)\<^sub>e )))
+   \<turnstile>\<^sub>r 
+    (L (Lv) ((reg\<^sup>> = reg\<^sup>< * 2 \<and> err\<^sup>> = 0)\<^sub>e ))
+  "
+  by (pred_auto_banks add: Lv_def DBL_def Loc_L_DBL_def)
+
+lemma 
+  assumes "V is VH"
+  shows "\<not>(L V (\<not>Pre\<^sup><)) = (\<forall> x \<Zspot> (V) \<longrightarrow> (Pre \<up> sys))"
+  apply pred_auto_banks
+
+lemma "(\<not>L (Lv) (\<not> ((reg\<^sup>< \<ge> 0 \<and> reg\<^sup>< \<le> 127 \<and> err\<^sup>< = 0)\<^sub>e ))) = false"
+  apply (subst L_def)
+  apply (pred_auto_banks add: Lv_def)
+  nitpick
+  
+
+lemma "Loc_L_DBL = true"
+  apply (subst loc_l_dbl_simp)
+  apply (subst Lv_def)
+  apply (subst L_def)
+  apply (pred_auto_banks add: Lv_def DBL_def Loc_L_DBL_def)
+   apply transfer
+   apply auto
+   
+
+
+
+declare [[smt_solver = cvc4]]
 (* TODO get H working *)
 
-(*
-lemma "Loc_H_DBL = (((vu:reg\<^sub>H\<^sup>< \<ge> 0 \<and> vu:reg\<^sub>H\<^sup>< \<le> 7 \<and> vu:err\<^sub>H\<^sup>< = 0)\<^sub>e  \<up> \<^bold>v\<^sub>D\<^sup>2)) \<turnstile> (((((vu:reg\<^sub>H\<^sup>> = vu:reg\<^sub>H\<^sup>< * 2) \<or> (vu:reg\<^sub>H\<^sup>> = (vu:reg\<^sub>H\<^sup>< * 2) + 1)) \<and> vu:err\<^sub>H\<^sup>> = 0)\<^sub>e \<up> \<^bold>v\<^sub>D\<^sup>2))"
-  apply (pred_auto_banks add: Hv_def DBL_def Loc_H_DBL_def)
-  sorry
-*)
+
+lemma "Loc_H_DBL = ((vu:reg\<^sub>H\<^sup>< \<ge> 0 \<and> vu:reg\<^sub>H\<^sup>< \<le> 7 \<and> vu:err\<^sub>H\<^sup>< = 0)\<^sub>e) \<turnstile>\<^sub>r (((vu:reg\<^sub>H\<^sup>> = vu:reg\<^sub>H\<^sup>< * 2) \<or> (vu:reg\<^sub>H\<^sup>> = (vu:reg\<^sub>H\<^sup>< * 2) + 1)) \<and> vu:err\<^sub>H\<^sup>> = 0)\<^sub>e"
+  apply (subst Loc_H_DBL_def)
+  apply (pred_auto_banks add: DBL_def Hv_def)
+             apply (simp add: drop_4_le_7_127)
+
+
+
 
 (* Attempt to split out a smaller proof *)
-(*
-lemma "((\<not>L\<^sub>D (Hv) (\<not> ((reg\<^sup>< \<ge> 0 \<and> reg\<^sup>< \<le> 127 \<and> err\<^sup>< = 0)\<^sub>e  \<up> \<^bold>v\<^sub>D\<^sup>2)))) = (((vu:reg\<^sub>H\<^sup>< \<ge> 0 \<and> vu:reg\<^sub>H\<^sup>< \<le> 7 \<and> vu:err\<^sub>H\<^sup>< = 0)\<^sub>e  \<up> \<^bold>v\<^sub>D\<^sup>2))"
+
+lemma "((\<not>L\<^sub>D (Hv) (\<not> ((reg\<^sup>< \<ge> 0 \<and> reg\<^sup>< \<le> 127 \<and> err\<^sup>< = 0)\<^sub>e  \<up> \<^bold>v\<^sub>D\<^sup>2)))) = ((vu:reg\<^sub>H\<^sup>< \<ge> 0 \<and> vu:reg\<^sub>H\<^sup>< \<le> 7 \<and> vu:err\<^sub>H\<^sup>< = 0)\<^sub>e  \<up> \<^bold>v\<^sub>D\<^sup>2)"
   apply (pred_auto_banks add: Hv_def)
-  sorry
-*)
-(*
+  defer
+  defer
+  quickcheck
+
+lemma "((\<not>L\<^sub>D (Hv) (\<not> ((reg\<^sup>< \<ge> 0 \<and> reg\<^sup>< \<le> 127 \<and> err\<^sup>< = 0)\<^sub>e  \<up> \<^bold>v\<^sub>D\<^sup>2)))) = true"
+  apply (subst L\<^sub>D_def)
+  apply (simp)
+  apply (subst \<Delta>\<^sub>D_def)
+  apply (subst to_viewed_design_def)
+  apply (simp)
+  apply (subst pair_map_def)
+  apply (subst Hv_def)+
+  apply (subst OK_def)+
+  apply (subst id_def)+
+  apply expr_simp
+  apply pred_simp
+  
+
 lemma "((L\<^sub>D (Hv) ((reg\<^sup>> = reg\<^sup>< * 2 \<and> err\<^sup>> = 0)\<^sub>e \<up> \<^bold>v\<^sub>D\<^sup>2))) = (((((vu:reg\<^sub>H\<^sup>> = vu:reg\<^sub>H\<^sup>< * 2) \<or> (vu:reg\<^sub>H\<^sup>> = (vu:reg\<^sub>H\<^sup>< * 2) + 1)) \<and> vu:err\<^sub>H\<^sup>> = 0)\<^sub>e \<up> \<^bold>v\<^sub>D\<^sup>2))"
   apply (pred_auto_banks add: Hv_def)
-  *)
+
 
 (* DBL2 doubles the number, if it is low enough to double without overflow, but unlike DBL, it
 explicitly defines the behaviour in the overflow case. If overflow is detected, then the err bit is
@@ -147,6 +222,37 @@ definition DBL2
 lemma "DBL \<sqsubseteq> DBL2"
   apply (pred_auto_banks add: DBL_def DBL2_def)
   by (transfer;auto)+
-    
 
+
+(* Increments the register value as long as it is less than 16 *)
+definition TestSys
+  where "TestSys = (
+    true
+    \<turnstile>\<^sub>r
+    (reg\<^sup>> = reg\<^sup>< + 1)\<^sub>e
+  )"
+
+definition Loc_L_TestSys where
+  "Loc_L_TestSys = L\<^sub>D (Lv) (TestSys)"
+
+
+
+lemma
+  fixes a :: "(('a \<alpha>ST_scheme, 'b \<alpha>L_scheme, 'c) viewed_system_scheme des_vars_ext * ('a \<alpha>ST_scheme, 'b \<alpha>L_scheme, 'c) viewed_system_scheme des_vars_ext)"
+  assumes "(to_viewed_design TestSys) a"
+  assumes "(\<Delta>\<^sub>D Lv) a"
+  shows "Loc_L_TestSys a = (true \<turnstile> ((vu:reg\<^sub>L\<^sup>> = (vu:reg\<^sub>L\<^sup>< + 1))\<^sub>e \<up> \<^bold>v\<^sub>D\<^sup>2)) a"
+  apply (subst Loc_L_TestSys_def)
+  apply (subst TestSys_def)
+  apply (subst Lv_def)
+  apply (subst L\<^sub>D_def)
+  apply (subst \<Delta>\<^sub>D_def)
+  apply (subst to_viewed_design_def)
+  apply simp
+  apply (subst pair_map_def)
+  apply expr_simp
+  apply pred_simp
+  (*apply (pred_auto_banks add: Loc_L_TestSys_def Lv_def TestSys_def)
+  quickcheck
+*)
 end
